\documentclass[UTF8,10pt,a4paper]{article}
\usepackage[vmargin=1in,hmargin=.5in]{geometry}
\usepackage{amsmath,amssymb,amsthm,bm}
\begin{document}
\begin{itemize}
\item For $u=x,\alpha=x,\beta=x$, we have
\small\begin{align}
\nonumber\chi_{\text{ED},xxx}^{(2)}=&\left(-\frac{\sqrt{3}}{2}\right)\left(-\frac{\sqrt{3}}{2}\right)\left(-\frac{\sqrt{3}}{2}\right)\chi_{\text{ED},yyy}^{(2)}\\
&+\left[\left(-\frac{1}{2}\right)\left(-\frac{1}{2}\right)\left(-\frac{\sqrt{3}}{2}\right)\chi_{\text{ED},xxy}^{(2)}\right]+\left[\left(-\frac{\sqrt{3}}{2}\right)\left(-\frac{1}{2}\right)\left(-\frac{1}{2}\right)\chi_{\text{ED},yxx}^{(2)}\right]+\left[\left(-\frac{1}{2}\right)\left(-\frac{\sqrt{3}}{2}\right)\left(-\frac{1}{2}\right)\chi_{\text{ED},xyx}^{(2)}\right]
\end{align}\normalsize
\item For $u=x,\alpha=x,\beta=y$, we have
\small\begin{align}
\nonumber\chi_{\text{ED},xxy}^{(2)}=&\left(-\frac{\sqrt{3}}{2}\right)\left(-\frac{\sqrt{3}}{2}\right)\left(-\frac{1}{2}\right)\chi_{\text{ED},yyy}^{(2)}\\
&+\left[\left(-\frac{1}{2}\right)\left(-\frac{1}{2}\right)\left(-\frac{1}{2}\right)\chi_{\text{ED},xxy}^{(2)}\right]+\left[\left(-\frac{\sqrt{3}}{2}\right)\left(-\frac{1}{2}\right)\frac{\sqrt{3}}{2}\chi_{\text{ED},yxx}^{(2)}\right]+\left[\left(-\frac{1}{2}\right)\left(-\frac{\sqrt{3}}{2}\right)\frac{\sqrt{3}}{2}\chi_{\text{ED},xyx}^{(2)}\right]
\end{align}\normalsize
\item For $u=x,\alpha=x,\beta=z$, we have
\small\begin{align}
\nonumber\chi_{\text{ED},xxz}^{(2)}=&\left(-\frac{\sqrt{3}}{2}\right)\left(-\frac{\sqrt{3}}{2}\right)1\chi_{\text{ED},yyz}^{(2)}\\
&+\left[\left(-\frac{1}{2}\right)\left(-\frac{1}{2}\right)1\chi_{\text{ED},xxz}^{(2)}\right]
\end{align}\normalsize
\item For $u=x,\alpha=y,\beta=x$, we have
\small\begin{align}
\nonumber\chi_{\text{ED},xyx}^{(2)}=&\left(-\frac{\sqrt{3}}{2}\right)\left(-\frac{1}{2}\right)\left(-\frac{\sqrt{3}}{2}\right)\chi_{\text{ED},yyy}^{(2)}\\
&+\left[\left(-\frac{1}{2}\right)\frac{\sqrt{3}}{2}\left(-\frac{\sqrt{3}}{2}\right)\chi_{\text{ED},xxy}^{(2)}\right]+\left[\left(-\frac{\sqrt{3}}{2}\right)\frac{\sqrt{3}}{2}\left(-\frac{1}{2}\right)\chi_{\text{ED},yxx}^{(2)}\right]+\left[\left(-\frac{1}{2}\right)\left(-\frac{1}{2}\right)\left(-\frac{1}{2}\right)\chi_{\text{ED},xyx}^{(2)}\right]
\end{align}\normalsize
\item For $u=x,\alpha=y,\beta=y$, we have
\small\begin{align}
\nonumber\chi_{\text{ED},xyy}^{(2)}=&\left(-\frac{\sqrt{3}}{2}\right)\left(-\frac{1}{2}\right)\left(-\frac{1}{2}\right)\chi_{\text{ED},yyy}^{(2)}\\
&+\left[\left(-\frac{1}{2}\right)\frac{\sqrt{3}}{2}\left(-\frac{1}{2}\right)\chi_{\text{ED},xxy}^{(2)}\right]+\left[\left(-\frac{\sqrt{3}}{2}\right)\frac{\sqrt{3}}{2}\frac{\sqrt{3}}{2}\chi_{\text{ED},yxx}^{(2)}\right]+\left[\left(-\frac{1}{2}\right)\left(-\frac{1}{2}\right)\frac{\sqrt{3}}{2}\chi_{\text{ED},xyx}^{(2)}\right]
\end{align}\normalsize
\item For $u=x,\alpha=y,\beta=z$, we have
\small\begin{align}
\nonumber\chi_{\text{ED},xyz}^{(2)}=&\left(-\frac{\sqrt{3}}{2}\right)\left(-\frac{1}{2}\right)1\chi_{\text{ED},yyz}^{(2)}\\
&+\left[\left(-\frac{1}{2}\right)\frac{\sqrt{3}}{2}1\chi_{\text{ED},xxz}^{(2)}\right]
\end{align}\normalsize
\item For $u=x,\alpha=z,\beta=x$, we have
\small\begin{align}
\nonumber\chi_{\text{ED},xzx}^{(2)}=&\left(-\frac{\sqrt{3}}{2}\right)1\left(-\frac{\sqrt{3}}{2}\right)\chi_{\text{ED},yzy}^{(2)}\\
&+\left[\left(-\frac{1}{2}\right)1\left(-\frac{1}{2}\right)\chi_{\text{ED},xzx}^{(2)}\right]
\end{align}\normalsize
\item For $u=x,\alpha=z,\beta=y$, we have
\small\begin{align}
\nonumber\chi_{\text{ED},xzy}^{(2)}=&\left(-\frac{\sqrt{3}}{2}\right)1\left(-\frac{1}{2}\right)\chi_{\text{ED},yzy}^{(2)}\\
&+\left[\left(-\frac{1}{2}\right)1\frac{\sqrt{3}}{2}\chi_{\text{ED},xzx}^{(2)}\right]
\end{align}\normalsize
\item For $u=x,\alpha=z,\beta=z$, we have
\small\begin{align}
\nonumber\chi_{\text{ED},xzz}^{(2)}=&\left(-\frac{\sqrt{3}}{2}\right)11\chi_{\text{ED},yzz}^{(2)}\\
&
\end{align}\normalsize
\item For $u=y,\alpha=x,\beta=x$, we have
\small\begin{align}
\nonumber\chi_{\text{ED},yxx}^{(2)}=&\left(-\frac{1}{2}\right)\left(-\frac{\sqrt{3}}{2}\right)\left(-\frac{\sqrt{3}}{2}\right)\chi_{\text{ED},yyy}^{(2)}\\
&+\left[\frac{\sqrt{3}}{2}\left(-\frac{1}{2}\right)\left(-\frac{\sqrt{3}}{2}\right)\chi_{\text{ED},xxy}^{(2)}\right]+\left[\left(-\frac{1}{2}\right)\left(-\frac{1}{2}\right)\left(-\frac{1}{2}\right)\chi_{\text{ED},yxx}^{(2)}\right]+\left[\frac{\sqrt{3}}{2}\left(-\frac{\sqrt{3}}{2}\right)\left(-\frac{1}{2}\right)\chi_{\text{ED},xyx}^{(2)}\right]
\end{align}\normalsize
\item For $u=y,\alpha=x,\beta=y$, we have
\small\begin{align}
\nonumber\chi_{\text{ED},yxy}^{(2)}=&\left(-\frac{1}{2}\right)\left(-\frac{\sqrt{3}}{2}\right)\left(-\frac{1}{2}\right)\chi_{\text{ED},yyy}^{(2)}\\
&+\left[\frac{\sqrt{3}}{2}\left(-\frac{1}{2}\right)\left(-\frac{1}{2}\right)\chi_{\text{ED},xxy}^{(2)}\right]+\left[\left(-\frac{1}{2}\right)\left(-\frac{1}{2}\right)\frac{\sqrt{3}}{2}\chi_{\text{ED},yxx}^{(2)}\right]+\left[\frac{\sqrt{3}}{2}\left(-\frac{\sqrt{3}}{2}\right)\frac{\sqrt{3}}{2}\chi_{\text{ED},xyx}^{(2)}\right]
\end{align}\normalsize
\item For $u=y,\alpha=x,\beta=z$, we have
\small\begin{align}
\nonumber\chi_{\text{ED},yxz}^{(2)}=&\left(-\frac{1}{2}\right)\left(-\frac{\sqrt{3}}{2}\right)1\chi_{\text{ED},yyz}^{(2)}\\
&+\left[\frac{\sqrt{3}}{2}\left(-\frac{1}{2}\right)1\chi_{\text{ED},xxz}^{(2)}\right]
\end{align}\normalsize
\item For $u=y,\alpha=y,\beta=x$, we have
\small\begin{align}
\nonumber\chi_{\text{ED},yyx}^{(2)}=&\left(-\frac{1}{2}\right)\left(-\frac{1}{2}\right)\left(-\frac{\sqrt{3}}{2}\right)\chi_{\text{ED},yyy}^{(2)}\\
&+\left[\frac{\sqrt{3}}{2}\frac{\sqrt{3}}{2}\left(-\frac{\sqrt{3}}{2}\right)\chi_{\text{ED},xxy}^{(2)}\right]+\left[\left(-\frac{1}{2}\right)\frac{\sqrt{3}}{2}\left(-\frac{1}{2}\right)\chi_{\text{ED},yxx}^{(2)}\right]+\left[\frac{\sqrt{3}}{2}\left(-\frac{1}{2}\right)\left(-\frac{1}{2}\right)\chi_{\text{ED},xyx}^{(2)}\right]
\end{align}\normalsize
\item For $u=y,\alpha=y,\beta=y$, we have
\small\begin{align}
\nonumber\chi_{\text{ED},yyy}^{(2)}=&\left(-\frac{1}{2}\right)\left(-\frac{1}{2}\right)\left(-\frac{1}{2}\right)\chi_{\text{ED},yyy}^{(2)}\\
&+\left[\frac{\sqrt{3}}{2}\frac{\sqrt{3}}{2}\left(-\frac{1}{2}\right)\chi_{\text{ED},xxy}^{(2)}\right]+\left[\left(-\frac{1}{2}\right)\frac{\sqrt{3}}{2}\frac{\sqrt{3}}{2}\chi_{\text{ED},yxx}^{(2)}\right]+\left[\frac{\sqrt{3}}{2}\left(-\frac{1}{2}\right)\frac{\sqrt{3}}{2}\chi_{\text{ED},xyx}^{(2)}\right]
\end{align}\normalsize
\item For $u=y,\alpha=y,\beta=z$, we have
\small\begin{align}
\nonumber\chi_{\text{ED},yyz}^{(2)}=&\left(-\frac{1}{2}\right)\left(-\frac{1}{2}\right)1\chi_{\text{ED},yyz}^{(2)}\\
&+\left[\frac{\sqrt{3}}{2}\frac{\sqrt{3}}{2}1\chi_{\text{ED},xxz}^{(2)}\right]
\end{align}\normalsize
\item For $u=y,\alpha=z,\beta=x$, we have
\small\begin{align}
\nonumber\chi_{\text{ED},yzx}^{(2)}=&\left(-\frac{1}{2}\right)1\left(-\frac{\sqrt{3}}{2}\right)\chi_{\text{ED},yzy}^{(2)}\\
&+\left[\frac{\sqrt{3}}{2}1\left(-\frac{1}{2}\right)\chi_{\text{ED},xzx}^{(2)}\right]
\end{align}\normalsize
\item For $u=y,\alpha=z,\beta=y$, we have
\small\begin{align}
\nonumber\chi_{\text{ED},yzy}^{(2)}=&\left(-\frac{1}{2}\right)1\left(-\frac{1}{2}\right)\chi_{\text{ED},yzy}^{(2)}\\
&+\left[\frac{\sqrt{3}}{2}1\frac{\sqrt{3}}{2}\chi_{\text{ED},xzx}^{(2)}\right]
\end{align}\normalsize
\item For $u=y,\alpha=z,\beta=z$, we have
\small\begin{align}
\nonumber\chi_{\text{ED},yzz}^{(2)}=&\left(-\frac{1}{2}\right)11\chi_{\text{ED},yzz}^{(2)}\\
&
\end{align}\normalsize
\item For $u=z,\alpha=x,\beta=x$, we have
\small\begin{align}
\nonumber\chi_{\text{ED},zxx}^{(2)}=&1\left(-\frac{\sqrt{3}}{2}\right)\left(-\frac{\sqrt{3}}{2}\right)\chi_{\text{ED},zyy}^{(2)}\\
&+\left[1\left(-\frac{1}{2}\right)\left(-\frac{1}{2}\right)\chi_{\text{ED},zxx}^{(2)}\right]
\end{align}\normalsize
\item For $u=z,\alpha=x,\beta=y$, we have
\small\begin{align}
\nonumber\chi_{\text{ED},zxy}^{(2)}=&1\left(-\frac{\sqrt{3}}{2}\right)\left(-\frac{1}{2}\right)\chi_{\text{ED},zyy}^{(2)}\\
&+\left[1\left(-\frac{1}{2}\right)\frac{\sqrt{3}}{2}\chi_{\text{ED},zxx}^{(2)}\right]
\end{align}\normalsize
\item For $u=z,\alpha=x,\beta=z$, we have
\small\begin{align}
\nonumber\chi_{\text{ED},zxz}^{(2)}=&1\left(-\frac{\sqrt{3}}{2}\right)1\chi_{\text{ED},zyz}^{(2)}\\
&
\end{align}\normalsize
\item For $u=z,\alpha=y,\beta=x$, we have
\small\begin{align}
\nonumber\chi_{\text{ED},zyx}^{(2)}=&1\left(-\frac{1}{2}\right)\left(-\frac{\sqrt{3}}{2}\right)\chi_{\text{ED},zyy}^{(2)}\\
&+\left[1\frac{\sqrt{3}}{2}\left(-\frac{1}{2}\right)\chi_{\text{ED},zxx}^{(2)}\right]
\end{align}\normalsize
\item For $u=z,\alpha=y,\beta=y$, we have
\small\begin{align}
\nonumber\chi_{\text{ED},zyy}^{(2)}=&1\left(-\frac{1}{2}\right)\left(-\frac{1}{2}\right)\chi_{\text{ED},zyy}^{(2)}\\
&+\left[1\frac{\sqrt{3}}{2}\frac{\sqrt{3}}{2}\chi_{\text{ED},zxx}^{(2)}\right]
\end{align}\normalsize
\item For $u=z,\alpha=y,\beta=z$, we have
\small\begin{align}
\nonumber\chi_{\text{ED},zyz}^{(2)}=&1\left(-\frac{1}{2}\right)1\chi_{\text{ED},zyz}^{(2)}\\
&
\end{align}\normalsize
\item For $u=z,\alpha=z,\beta=x$, we have
\small\begin{align}
\nonumber\chi_{\text{ED},zzx}^{(2)}=&11\left(-\frac{\sqrt{3}}{2}\right)\chi_{\text{ED},zzy}^{(2)}\\
&
\end{align}\normalsize
\item For $u=z,\alpha=z,\beta=y$, we have
\small\begin{align}
\nonumber\chi_{\text{ED},zzy}^{(2)}=&11\left(-\frac{1}{2}\right)\chi_{\text{ED},zzy}^{(2)}\\
&
\end{align}\normalsize
\item For $u=z,\alpha=z,\beta=z$, we have
\small\begin{align}
\nonumber\chi_{\text{ED},zzz}^{(2)}=&111\chi_{\text{ED},zzz}^{(2)}\\
&
\end{align}\normalsize
\end{itemize}
\end{document}